02_FORMAL/lean/lakefile.lean
@@ -3,7 +3,6 @@ open Lake DSL
 
 -- Copyright (c) 2026 The RIINA Authors. All rights reserved.
 -- RIINA Formal Proofs - Lean 4 Port
--- Multi-prover verification port from Coq originals.
 
 package RIINA where
   version := v!"0.2.0"
